theories/iris/logrel/env_props.v
@@ -1,0 +1,212 @@
+Require Import RecordUpdate.RecordUpdate.
+Require Import RichWasm.iris.language.iris_wp_def.
+Require Import RichWasm.iris.logrel.
+Require Import RichWasm.layout.
+Require Import RichWasm.syntax.
+Require Import RichWasm.typing.
+Set Bullet Behavior "Strict Subproofs".
+Set Default Goal Selector "!".
+
+Section env_props.
+
+  Context `{!logrel_na_invs Σ}.
+  Context `{!wasmG Σ}.
+  Context `{!richwasmG Σ}.
+
+
+  Lemma eval_rep_mem_irrel_eq se ρ μ :
+    eval_rep se ρ =
+    eval_rep (senv_insert_mem (Σ:=Σ) μ se) ρ.
+  Proof.
+    induction ρ using rep_ind; auto.
+    - cbn in *.
+      assert (H': mapM (eval_rep se) ρs = mapM (eval_rep (senv_insert_mem μ se)) ρs)
+        by by apply Forall_mapM_ext.
+      by rewrite H'.
+    - cbn in *.
+      assert (H': mapM (eval_rep se) ρs = mapM (eval_rep (senv_insert_mem μ se)) ρs)
+        by by apply Forall_mapM_ext.
+      by rewrite H'.
+  Qed.
+
+  Lemma eval_rep_mem_irrel se ρ ιs μ :
+    eval_rep se ρ = Some ιs ->
+    eval_rep (senv_insert_mem (Σ:=Σ) μ se) ρ = Some ιs.
+  Proof.
+    intros; rewrite <- eval_rep_mem_irrel_eq; done.
+  Qed.
+
+  Lemma eval_rep_size_irrel_eq se ρ n :
+    eval_rep se ρ =
+    eval_rep (senv_insert_size (Σ:=Σ) n se) ρ.
+  Proof.
+    induction ρ using rep_ind; auto.
+    - cbn in *.
+      assert (H': mapM (eval_rep se) ρs = mapM (eval_rep (senv_insert_size n se)) ρs)
+        by by apply Forall_mapM_ext.
+      by rewrite H'.
+    - cbn in *.
+      assert (H': mapM (eval_rep se) ρs = mapM (eval_rep (senv_insert_size n se)) ρs)
+        by by apply Forall_mapM_ext.
+      by rewrite H'.
+  Qed.
+
+  Lemma eval_rep_size_irrel se ρ ιs n :
+    eval_rep se ρ = Some ιs ->
+    eval_rep (senv_insert_size (Σ:=Σ) n se) ρ = Some ιs.
+  Proof.
+    intros; rewrite <- eval_rep_size_irrel_eq; done.
+  Qed.
+
+  Lemma eval_rep_type_irrel_eq se ρ sκ sκ_T T :
+    eval_rep se ρ =
+    eval_rep (senv_insert_type (Σ:=Σ) sκ sκ_T T se) ρ.
+  Proof.
+    induction ρ using rep_ind; auto.
+    - cbn in *.
+      assert (H': mapM (eval_rep se) ρs = mapM (eval_rep (senv_insert_type sκ sκ_T T se)) ρs)
+        by by apply Forall_mapM_ext.
+      by rewrite H'.
+    - cbn in *.
+      assert (H': mapM (eval_rep se) ρs = mapM (eval_rep (senv_insert_type sκ sκ_T T se)) ρs)
+        by by apply Forall_mapM_ext.
+      by rewrite H'.
+  Qed.
+
+  Lemma eval_rep_type_irrel se ρ ιs sκ sκ_T T :
+    eval_rep se ρ = Some ιs ->
+    eval_rep (senv_insert_type (Σ:=Σ) sκ sκ_T T se) ρ = Some ιs.
+  Proof.
+    intros; rewrite <- eval_rep_type_irrel_eq; done.
+  Qed.
+
+  Lemma eval_size_mem_irrel_eq se σ μ :
+    eval_size se σ =
+    eval_size (senv_insert_mem (Σ:=Σ) μ se) σ.
+  Proof.
+    induction σ using size_ind; intros; auto.
+    - cbn in *.
+      assert (H': mapM (eval_size se) σs = mapM (eval_size (senv_insert_mem μ se)) σs)
+        by by apply Forall_mapM_ext.
+      by rewrite H'.
+    - cbn in *.
+      assert (H': mapM (eval_size se) σs = mapM (eval_size (senv_insert_mem μ se)) σs)
+        by by apply Forall_mapM_ext.
+      by rewrite H'.
+    - cbn -[senv_insert_mem].
+      by rewrite <- eval_rep_mem_irrel_eq.
+  Qed.
+
+  Lemma eval_size_mem_irrel se σ n μ :
+    eval_size se σ = Some n ->
+    eval_size (senv_insert_mem (Σ:=Σ) μ se) σ = Some n.
+  Proof.
+    intros; rewrite <- eval_size_mem_irrel_eq; done.
+  Qed.
+
+  Lemma eval_size_type_irrel_eq se σ sκ sκ_T T :
+    eval_size se σ =
+    eval_size (senv_insert_type (Σ:=Σ) sκ sκ_T T se) σ.
+  Proof.
+    induction σ using size_ind; intros; auto.
+    - cbn in *.
+      assert (H': mapM (eval_size se) σs = mapM (eval_size (senv_insert_type sκ sκ_T T se)) σs)
+        by by apply Forall_mapM_ext.
+      by rewrite H'.
+    - cbn in *.
+      assert (H': mapM (eval_size se) σs = mapM (eval_size (senv_insert_type sκ sκ_T T se)) σs)
+        by by apply Forall_mapM_ext.
+      by rewrite H'.
+    - cbn -[senv_insert_type].
+      by rewrite <- eval_rep_type_irrel_eq.
+  Qed.
+
+  Lemma eval_size_type_irrel se σ n sκ sκ_T T :
+    eval_size se σ = Some n ->
+    eval_size (senv_insert_type (Σ:=Σ) sκ sκ_T T se) σ = Some n.
+  Proof.
+    intros; rewrite <- eval_size_type_irrel_eq; done.
+  Qed.
+
+  Lemma eval_mem_type_irrel_eq se m sκ sκ_T T :
+    eval_mem se m =
+    eval_mem (senv_insert_type (Σ:=Σ) sκ sκ_T T se) m.
+  Proof.
+    destruct m; auto.
+  Qed.
+
+  Lemma eval_kind_mem_irrel_eq se κ μ :
+    eval_kind se κ =
+    eval_kind (senv_insert_mem (Σ:=Σ) μ se) κ .
+  Proof.
+    destruct κ; intros; cbn -[senv_insert_mem senv_insert_type] in *.
+    - by rewrite <- eval_rep_mem_irrel_eq.
+    - by rewrite <- eval_size_mem_irrel_eq.
+  Qed.
+
+  Lemma eval_kind_mem_irrel se κ sκ μ :
+    eval_kind se κ = Some sκ ->
+    eval_kind (senv_insert_mem (Σ:=Σ) μ se) κ = Some sκ.
+  Proof.
+    intros; rewrite <- eval_kind_mem_irrel_eq; done.
+  Qed.
+
+  Lemma eval_kind_type_irrel_eq se κ sκ sκ_T T :
+    eval_kind se κ =
+    eval_kind (senv_insert_type (Σ:=Σ) sκ sκ_T T se) κ .
+  Proof.
+    destruct κ; intros; cbn -[senv_insert_type] in *.
+    - by rewrite <- eval_rep_type_irrel_eq.
+    - by rewrite <- eval_size_type_irrel_eq.
+  Qed.
+
+  Lemma eval_kind_type_irrel se κ sκ sκ' sκ_T T :
+    eval_kind se κ = Some sκ ->
+    eval_kind (senv_insert_type (Σ:=Σ) sκ' sκ_T T se) κ = Some sκ.
+  Proof.
+    intros; rewrite <- eval_kind_type_irrel_eq; done.
+  Qed.
+
+  Lemma type_skind_mem_irrel_eq se μ τ :
+    type_skind (Σ:=Σ) se τ =
+    type_skind (Σ:=Σ) (senv_insert_mem μ se)
+      (ren_type unscoped.shift unscoped.id unscoped.id unscoped.id τ).
+  Proof.
+    destruct τ.
+    1: done.
+    all: intros; cbn in *.
+    all: rewrite rinstId'_kind.
+    all: by apply eval_kind_mem_irrel_eq.
+  Qed.
+
+  Lemma type_skind_mem_irrel se μ τ sκ :
+    type_skind (Σ:=Σ) se τ = Some sκ ->
+    type_skind (Σ:=Σ) (senv_insert_mem μ se)
+      (ren_type unscoped.shift unscoped.id unscoped.id unscoped.id τ) = Some sκ.
+  Proof.
+    intros; rewrite <- type_skind_mem_irrel_eq; done.
+  Qed.
+
+  Lemma sem_env_interp_insert_type F (se : semantic_env (Σ:=Σ)) κ sκ sκ_T T :
+    sem_env_interp F se →
+    eval_kind se κ = Some sκ →
+    subskind_of sκ_T sκ ->
+    skind_has_stype sκ_T T →
+    sem_env_interp (F <| fc_type_vars ::= cons κ |>) (senv_insert_type sκ sκ_T T se).
+  Proof.
+    intros [Hkind Htypes] Hκ Hsubsk HT.
+    split.
+    - destruct Hkind as (Hmem & Hrep & Hsize).
+      repeat split; cbn; done.
+    - cbn [fc_type_vars].
+      apply Forall2_cons.
+      split.
+      + split.
+        * by eapply eval_kind_type_irrel.
+        * done.
+      + eapply Forall2_impl; [exact Htypes|].
+        intros κ' [sκ' [sκ_T' T']] [Heval' HT'].
+        split; [by eapply eval_kind_type_irrel | exact HT'].
+  Qed.
+
+End env_props.
