theories/iris/logrel/instr/typing/inst.v
@@ -1,5 +1,6 @@
 Require Import RichWasm.iris.logrel.instr.typing.common.
 Require Import RichWasm.iris.logrel.logrel_properties.
+Require Import RichWasm.iris.logrel.env_props.
 Set Bullet Behavior "Strict Subproofs".
 Set Default Goal Selector "!".
 
@@ -272,179 +273,6 @@ Admitted.
       apply Forall2_fmap;
       eapply Forall2_mini_impl_Forall; first done;
       done.
-
-  Lemma eval_rep_mem_irrel_eq se ρ μ :
-    eval_rep se ρ =
-    eval_rep (senv_insert_mem (Σ:=Σ) μ se) ρ.
-  Proof.
-    induction ρ using rep_ind; auto.
-    - cbn in *.
-      assert (H': mapM (eval_rep se) ρs = mapM (eval_rep (senv_insert_mem μ se)) ρs)
-        by by apply Forall_mapM_ext.
-      by rewrite H'.
-    - cbn in *.
-      assert (H': mapM (eval_rep se) ρs = mapM (eval_rep (senv_insert_mem μ se)) ρs)
-        by by apply Forall_mapM_ext.
-      by rewrite H'.
-  Qed.
-
-  Lemma eval_rep_mem_irrel se ρ ιs μ :
-    eval_rep se ρ = Some ιs ->
-    eval_rep (senv_insert_mem (Σ:=Σ) μ se) ρ = Some ιs.
-  Proof.
-    intros; rewrite <- eval_rep_mem_irrel_eq; done.
-  Qed.
-
-  Lemma eval_rep_size_irrel_eq se ρ n :
-    eval_rep se ρ =
-    eval_rep (senv_insert_size (Σ:=Σ) n se) ρ.
-  Proof.
-    induction ρ using rep_ind; auto.
-    - cbn in *.
-      assert (H': mapM (eval_rep se) ρs = mapM (eval_rep (senv_insert_size n se)) ρs)
-        by by apply Forall_mapM_ext.
-      by rewrite H'.
-    - cbn in *.
-      assert (H': mapM (eval_rep se) ρs = mapM (eval_rep (senv_insert_size n se)) ρs)
-        by by apply Forall_mapM_ext.
-      by rewrite H'.
-  Qed.
-
-  Lemma eval_rep_size_irrel se ρ ιs n :
-    eval_rep se ρ = Some ιs ->
-    eval_rep (senv_insert_size (Σ:=Σ) n se) ρ = Some ιs.
-  Proof.
-    intros; rewrite <- eval_rep_size_irrel_eq; done.
-  Qed.
-
-  Lemma eval_rep_type_irrel_eq se ρ sκ sκ_T T :
-    eval_rep se ρ =
-    eval_rep (senv_insert_type (Σ:=Σ) sκ sκ_T T se) ρ.
-  Proof.
-    induction ρ using rep_ind; auto.
-    - cbn in *.
-      assert (H': mapM (eval_rep se) ρs = mapM (eval_rep (senv_insert_type sκ sκ_T T se)) ρs)
-        by by apply Forall_mapM_ext.
-      by rewrite H'.
-    - cbn in *.
-      assert (H': mapM (eval_rep se) ρs = mapM (eval_rep (senv_insert_type sκ sκ_T T se)) ρs)
-        by by apply Forall_mapM_ext.
-      by rewrite H'.
-  Qed.
-
-  Lemma eval_rep_type_irrel se ρ ιs sκ sκ_T T :
-    eval_rep se ρ = Some ιs ->
-    eval_rep (senv_insert_type (Σ:=Σ) sκ sκ_T T se) ρ = Some ιs.
-  Proof.
-    intros; rewrite <- eval_rep_type_irrel_eq; done.
-  Qed.
-
-  Lemma eval_size_mem_irrel_eq se σ μ :
-    eval_size se σ =
-    eval_size (senv_insert_mem (Σ:=Σ) μ se) σ.
-  Proof.
-    induction σ using size_ind; intros; auto.
-    - cbn in *.
-      assert (H': mapM (eval_size se) σs = mapM (eval_size (senv_insert_mem μ se)) σs)
-        by by apply Forall_mapM_ext.
-      by rewrite H'.
-    - cbn in *.
-      assert (H': mapM (eval_size se) σs = mapM (eval_size (senv_insert_mem μ se)) σs)
-        by by apply Forall_mapM_ext.
-      by rewrite H'.
-    - cbn -[senv_insert_mem].
-      by rewrite <- eval_rep_mem_irrel_eq.
-  Qed.
-
-  Lemma eval_size_mem_irrel se σ n μ :
-    eval_size se σ = Some n ->
-    eval_size (senv_insert_mem (Σ:=Σ) μ se) σ = Some n.
-  Proof.
-    intros; rewrite <- eval_size_mem_irrel_eq; done.
-  Qed.
-
-  Lemma eval_size_type_irrel_eq se σ sκ sκ_T T :
-    eval_size se σ =
-    eval_size (senv_insert_type (Σ:=Σ) sκ sκ_T T se) σ.
-  Proof.
-    induction σ using size_ind; intros; auto.
-    - cbn in *.
-      assert (H': mapM (eval_size se) σs = mapM (eval_size (senv_insert_type sκ sκ_T T se)) σs)
-        by by apply Forall_mapM_ext.
-      by rewrite H'.
-    - cbn in *.
-      assert (H': mapM (eval_size se) σs = mapM (eval_size (senv_insert_type sκ sκ_T T se)) σs)
-        by by apply Forall_mapM_ext.
-      by rewrite H'.
-    - cbn -[senv_insert_type].
-      by rewrite <- eval_rep_type_irrel_eq.
-  Qed.
-
-  Lemma eval_size_type_irrel se σ n sκ sκ_T T :
-    eval_size se σ = Some n ->
-    eval_size (senv_insert_type (Σ:=Σ) sκ sκ_T T se) σ = Some n.
-  Proof.
-    intros; rewrite <- eval_size_type_irrel_eq; done.
-  Qed.
-
-  Lemma eval_mem_type_irrel_eq se m sκ sκ_T T :
-    eval_mem se m =
-    eval_mem (senv_insert_type (Σ:=Σ) sκ sκ_T T se) m.
-  Proof.
-    destruct m; auto.
-  Qed.
-
-  Lemma eval_kind_mem_irrel_eq se κ μ :
-    eval_kind se κ =
-    eval_kind (senv_insert_mem (Σ:=Σ) μ se) κ .
-  Proof.
-    destruct κ; intros; cbn -[senv_insert_mem senv_insert_type] in *.
-    - by rewrite <- eval_rep_mem_irrel_eq.
-    - by rewrite <- eval_size_mem_irrel_eq.
-  Qed.
-
-  Lemma eval_kind_mem_irrel se κ sκ μ :
-    eval_kind se κ = Some sκ ->
-    eval_kind (senv_insert_mem (Σ:=Σ) μ se) κ = Some sκ.
-  Proof.
-    intros; rewrite <- eval_kind_mem_irrel_eq; done.
-  Qed.
-
-  Lemma eval_kind_type_irrel_eq se κ sκ sκ_T T :
-    eval_kind se κ =
-    eval_kind (senv_insert_type (Σ:=Σ) sκ sκ_T T se) κ .
-  Proof.
-    destruct κ; intros; cbn -[senv_insert_type] in *.
-    - by rewrite <- eval_rep_type_irrel_eq.
-    - by rewrite <- eval_size_type_irrel_eq.
-  Qed.
-
-  Lemma eval_kind_type_irrel se κ sκ sκ' sκ_T T :
-    eval_kind se κ = Some sκ ->
-    eval_kind (senv_insert_type (Σ:=Σ) sκ' sκ_T T se) κ = Some sκ.
-  Proof.
-    intros; rewrite <- eval_kind_type_irrel_eq; done.
-  Qed.
-
-  Lemma type_skind_mem_irrel_eq se μ τ :
-    type_skind (Σ:=Σ) se τ =
-    type_skind (Σ:=Σ) (senv_insert_mem μ se)
-      (ren_type unscoped.shift unscoped.id unscoped.id unscoped.id τ).
-  Proof.
-    destruct τ.
-    1: done.
-    all: intros; cbn in *.
-    all: rewrite rinstId'_kind.
-    all: by apply eval_kind_mem_irrel_eq.
-  Qed.
-
-  Lemma type_skind_mem_irrel se μ τ sκ :
-    type_skind (Σ:=Σ) se τ = Some sκ ->
-    type_skind (Σ:=Σ) (senv_insert_mem μ se)
-      (ren_type unscoped.shift unscoped.id unscoped.id unscoped.id τ) = Some sκ.
-  Proof.
-    intros; rewrite <- type_skind_mem_irrel_eq; done.
-  Qed.
 
   Lemma Forall_mapM_map_ext {A B:Type} (f g:A → option B) h (l: list A) :
     Forall (λ x, f x = g (h x)) l -> mapM f l = mapM g (map h l).
@@ -1417,30 +1245,7 @@ Admitted.
       done.
   Admitted.
 
-  Lemma sem_env_interp_insert_type F (se : semantic_env (Σ:=Σ)) κ sκ sκ_T T :
-    sem_env_interp F se →
-    eval_kind se κ = Some sκ →
-    subskind_of sκ_T sκ ->
-    skind_has_stype sκ_T T →
-    sem_env_interp (F <| fc_type_vars ::= cons κ |>) (senv_insert_type sκ sκ_T T se).
-  Proof.
-    intros [Hkind Htypes] Hκ Hsubsk HT.
-    split.
-    - destruct Hkind as (Hmem & Hrep & Hsize).
-      repeat split; cbn; done.
-    - cbn [fc_type_vars].
-      apply Forall2_cons.
-      split.
-      + split.
-        * by eapply eval_kind_type_irrel.
-        * done.
-      + eapply Forall2_impl; [exact Htypes|].
-        intros κ' [sκ' [sκ_T' T']] [Heval' HT'].
-        split; [by eapply eval_kind_type_irrel | exact HT'].
-  Qed.
-
-  (* NOT DONE P:H, THIS IS *THE* LEMMA TO WORRY ABOUT *)
-  (* I think it's fine. But who knows. *)
+  (* the big scary one *)
   Lemma skind_interp_chillin :
     ∀ τ F F' κ κ' (se:semantic_env (Σ:=Σ)) se' sub_m sub_r sub_s sub_t sv,
     let τ' := refresh_kinds F (subst_type sub_m sub_r sub_s sub_t τ) in
@@ -2979,7 +2784,8 @@ Admitted.
         destruct y.
         intros.
         change (b::se.1.1.1, se.1.1.2, se.1.2, se.2) with (senv_insert_mem b se).
-        rewrite <- eval_kind_mem_irrel_eq.
+        destruct p.
+        rewrite <- (@eval_kind_mem_irrel_eq Σ).
         done.
   Qed.
 
@@ -3172,7 +2978,7 @@ Admitted.
       apply Forall2_cons.
       split.
       + change (se.1, (sκ, (sκ_T, T))::se.2) with (senv_insert_type sκ sκ_T T se).
-        rewrite <- eval_kind_type_irrel_eq.
+        rewrite <- (@eval_kind_type_irrel_eq Σ).
         try done.
       + unfold type_ctx_interp in h2.
         eapply Forall2_impl; first exact h2.
@@ -3180,7 +2986,7 @@ Admitted.
         destruct y.
         intros.
         change (se.1, (sκ, (sκ_T, T))::se.2) with (senv_insert_type sκ sκ_T T se).
-        rewrite <- eval_kind_type_irrel_eq.
+        rewrite <- (@eval_kind_type_irrel_eq Σ).
         done.
     - done.
     - done.
